theories/Operational/Common/OSAlgorithmAdapterContract.v
@@ -1,0 +1,89 @@
+From RocqSched Require Import Foundation.Base.
+From RocqSched Require Import Abstractions.SchedulingAlgorithm.Interface.
+From RocqSched Require Import Abstractions.SchedulingAlgorithm.SchedulerBridge.
+From RocqSched Require Import Abstractions.SchedulingAlgorithm.TopMInterface.
+From RocqSched Require Import Multicore.Common.MultiCoreBase.
+From RocqSched Require Import Multicore.Common.Admissibility.
+From RocqSched Require Import Multicore.Common.AdmissibleCandidateSource.
+From RocqSched Require Import Operational.Common.OSProjectionInterface.
+From RocqSched Require Import Operational.Common.OSSchedulerRelationContract.
+
+Record os_single_cpu_algorithm_adapter_contract
+    {CState : Type}
+    (P : OSLabeledProjection CState)
+    (J : JobId -> Prop)
+    (spec : GenericSchedulingAlgorithm)
+    (candidates_of : CandidateSource)
+    (jobs : JobId -> Job)
+    (adm : admissible_cpu) : Type :=
+  mkOSSingleCPUAlgorithmAdapterContract {
+    osaac_scheduler_relation :
+      os_local_single_cpu_scheduler_relation_adapter_contract
+        P
+        spec
+        candidates_of
+        jobs
+        adm;
+    osaac_candidate_source_spec :
+      CandidateSourceSpec J candidates_of;
+  }.
+
+Arguments osaac_scheduler_relation
+  {CState P J spec candidates_of jobs adm} _.
+Arguments osaac_candidate_source_spec
+  {CState P J spec candidates_of jobs adm} _.
+
+Record os_top_m_algorithm_adapter_contract
+    {CState : Type}
+    (P : OSLabeledProjection CState)
+    (J : JobId -> Prop)
+    (spec : GenericTopMSchedulingAlgorithm)
+    (candidates_of : CandidateSource)
+    (jobs : JobId -> Job)
+    (adm : admissible_cpu)
+    (m : nat) : Type :=
+  mkOSTopMAlgorithmAdapterContract {
+    otmaac_scheduler_relation :
+      os_local_top_m_scheduler_relation_adapter_contract
+        P
+        spec
+        candidates_of
+        jobs
+        adm
+        m;
+    otmaac_candidate_source_spec :
+      AdmissibleCandidateSourceSpec adm J candidates_of;
+  }.
+
+Arguments otmaac_scheduler_relation
+  {CState P J spec candidates_of jobs adm m} _.
+Arguments otmaac_candidate_source_spec
+  {CState P J spec candidates_of jobs adm m} _.
+
+Record os_strong_top_m_algorithm_adapter_contract
+    {CState : Type}
+    (P : OSLabeledProjection CState)
+    (J : JobId -> Prop)
+    (spec : GenericTopMSchedulingAlgorithm)
+    (candidates_of : CandidateSource)
+    (jobs : JobId -> Job)
+    (adm : admissible_cpu)
+    (m : nat) : Type :=
+  mkOSStrongTopMAlgorithmAdapterContract {
+    ostmaac_base :
+      os_top_m_algorithm_adapter_contract
+        P
+        J
+        spec
+        candidates_of
+        jobs
+        adm
+        m;
+    ostmaac_candidate_source_spec :
+      StrongAdmissibleCandidateSourceSpec adm J candidates_of;
+  }.
+
+Arguments ostmaac_base
+  {CState P J spec candidates_of jobs adm m} _.
+Arguments ostmaac_candidate_source_spec
+  {CState P J spec candidates_of jobs adm m} _.
